test/coq/incr_proof.v
@@ -9,7 +9,7 @@ From iris Require Import base_logic.lib.gen_heap.
 From osiris Require Import base.
 From osiris.lang Require Import lang encode.
 From osiris.semantics Require Import sugar locations free eval step notations.
-From osiris.weakestpre Require Import wp wp_tactics notations.
+From osiris.weakestpre Require Import wp wp_tactics notations safe.
 From osiris.libs Require Import Stdlib.
 From test Require Import incr.
 
@@ -51,206 +51,112 @@ Definition thirteen_spec v : iProp Σ :=
   ⌜ v = encode 13 ⌝.
 
 
-
-Definition spec_env : Type :=
-  gmap var (val → iProp Σ).
-
-Definition module_spec_env (Λ : spec_env) (η: env) : iProp Σ :=
-  ∀ x,
-  ∃ φ, ⌜Λ !! x = Some φ⌝ -∗
-       ∃ v, ⌜lookup_name η x = Ret v⌝ -∗
-       φ v.
-
-
-Definition module_spec (Λ : spec_env) (v: val) : iProp Σ :=
-  ∃ η, ⌜ v = VStruct η ⌝ ∗ module_spec_env Λ η.
-
-
-Implicit Type Λ : spec_env.
-Implicit Type η : env.
-Implicit Type x : var.
-Implicit Type e : expr.
-
-Definition module_spec_delete x Λ :=
-  let φ : val → iProp Σ := λ _, ⌜False⌝%I in
-  <[ x := φ ]> Λ.
-
-
-Lemma module_spec_ILet_now Λ η x e (t: list sitem) φx :
-  Λ !! x = Some φx →
-  let Λx := module_spec_delete x Λ in
-  ⊢ WP eval η e {{ φx }} -∗
-    (∀ v, φx v -∗
-      WP eval_mexpr (EnvCons x v η) (MkStruct t) {{ module_spec Λx }}) -∗
-    WP eval_mexpr η (MkStruct (ILet (Binding1 (PVar x) e) :: t))
-    {{ module_spec Λ }}.
-Proof.
-  iIntros (Hsome Λx) "He Ht".
-  wp.
-  iApply (wp_covariant with "He").
-  iIntros (v) "Hv".
-  iSpecialize ("Ht" with "Hv").
-Admitted.
-
-Lemma Incr__spec s E:
+Lemma Incr__spec:
   let Λ :=
-    {[
-      "new_counter" := new_counter_spec;
-      "test" := thirteen_spec
-    ]}
+    [
+      ("new_counter", new_counter_spec);
+      ("_test", thirteen_spec)
+    ]
   in
   let η := EnvCons "Stdlib" Stdlib $
            EnvNil in
-  ⊢ WP eval_mexpr η Incr @ s; E {{ module_spec Λ }}.
+  ⊢ WP eval_mexpr η Incr {{ module_spec Λ }}.
 Proof.
-  intros.
-  unfold Incr.
-  iStartProof.
-  remember (EFun1Pat _ _).
-  remember (Binding1 PAny _).
-  remember (Binding1 (PVar "_test") (ELet _ _)).
-
-  wp.
-  wp_call.
-  iApply wp_covariant; first by iApply Stdlib__ref__spec.
-  iIntros (?)"(%l&Hl&->)".
-  wp.
-  iPoseProof (Stdlib__snd__spec_tac with "[//][Hl]") as "H"; last iAssumption.
-  wp.
-  wp_call.
-  iApply (Stdlib__load__spec_tac with "[//]Hl").
-  iIntros "Hl".
-  wp.
-  iApply (Stdlib__store__spec_tac with "Hl").
-  wp.
-  iIntros "Hl".
-  wp.
-  wp_call.
-  iApply (Stdlib__load__spec_tac with "[//]Hl").
-  iIntros "Hl".
-  wp.
-  iApply (Stdlib__store__spec_tac with "Hl").
-
-
-
-(* --------------------------------------------------------------------------- *)
-(* Proof of the program. *)
-
-Lemma new_counter__spec s E :
-  let η := EnvCons "Stdlib" Stdlib $
-           EnvNil in
-  ⊢ WP eval η new_counter @ s; E
-       {{ λ v, {{{ ⌜ True ⌝ }}}
-                 call v VUnit
-               {{{ vget vupd,
-                     RET (VTuple (VCons vget (VCons vupd VNil)));
-                   ∃ ℓ,
-                   is_counter ℓ 0 ∗
-                   get_spec ℓ vget ∗
-                   upd_spec ℓ vupd }}} }}.
-Proof.
-  intros. wp.
-  iIntros (ϕ) "!> _ Hϕ".
-  wp_call.
-
-  (* TODO: fix the proof ([Stdlib__ref__spec_tac] should be applicable instead
-     of using [wp_covariant]). *)
-  iApply wp_covariant; first by iApply Stdlib__ref__spec.
-  iIntros (?) "(%ℓ&Hℓ&->)".
-  wp. iApply "Hϕ". clear ϕ.
-  iExists ℓ.
-  iSplitL; last iSplit.
-
-  { (* Proof of the [is_counter] predicate. *)
-    unfold is_counter. iExists _. by iFrame. }
-
-  { (* Proving the specification of [get]. *)
-    unfold get_spec. iIntros.
-    iIntros(ϕ)"!>(%&->&Hℓ) Hϕ".
-    wp_call. wp.
-
-    iApply (Stdlib__load__spec_tac $! ϕ with "[//]Hℓ").
-
-    iIntros "Hℓ".
-    iApply "Hϕ".
-    iSplit; first done.
-    iExists _; by iFrame. }
-
-
-  { (* Proof of the specification of [upd]. *)
-    unfold upd_spec. iIntros.
-    iIntros (ϕ) "!>(%&->&Hℓ) Hϕ".
-    wp_call.
-    iApply (Stdlib__store__spec_tac with "Hℓ[Hϕ]").
-    iNext.
-    iIntros "Hℓ".
-    iApply "Hϕ".
-    iExists _. by iFrame. }
-Qed.
-
-
-(* The following example shows issues in the standart library :
-   - arithmetic operators should *not* require user interactions at all.
-     TODO: write clean lemmas about totally applied ["Stdlib"."+"] and al. and
-           add them to a hint database.
-*)
-Opaque new_counter.
-Lemma pleasedontclash__spec :
-  let η :=
-    EnvCons "Stdlib" Stdlib $
-    EnvNil in
-  {{{ ⌜ True ⌝ }}}
-    eval η pleasedontclash
-  {{{ v, RET v; ⌜ v = VInt (int.repr 13) ⌝ }}}.
-Proof.
-  iIntros (η ϕ)"_ Hϕ".
+  iIntros.
   wp.
 
-  (* Fetch the specification of [new_counter] proven above.
-     TODO: better handle the use of recent definitions. *)
-  pose proof (new_counter__spec) as Hspec; simpl in Hspec;
-    iPoseProof Hspec as "#Hspec". clear Hspec.
+  (* Prove that [new_counter] matches its specification (defined above). *)
+  wp_specify "new_counter" new_counter_spec.
+  { iIntros (φ) "!>_ Hφ".
+    wp_call. wp_continue.
+    iApply wp_covariant; first by iApply Stdlib__ref__spec.
+    iIntros (?) "(%ℓ&Hℓ&->)".
+    wp_autocontinue. wp_use "Hφ". clear φ.
+    iExists ℓ.
+    iSplitL; last iSplit.
+    { (* Proof of the [is_counter] predicate. *)
+      unfold is_counter. iExists _. by iFrame. }
 
-  (* Use the aforementioned specification to get the value to which
-     [new_counter] evaluates and its specification. *)
-  iApply (wp_covariant with "Hspec").
-  iIntros (vnew_counter)"#Hnew_counter_spec".
+    { (* Proving the specification of [get]. *)
+      unfold get_spec. iIntros.
+      iIntros(ϕ)"!>(%&->&Hℓ) Hϕ".
+      wp_call. wp_autocontinue.
 
-  (* I avoid using tactics from [wp_tactics.v] not to reduce under
-     continuations anymore. *)
-  wp.
-  iApply ("Hnew_counter_spec" with "[//][Hϕ]").
+      iApply (Stdlib__load__spec_tac $! ϕ with "[//]Hℓ").
 
-  iNext. iIntros (vget vupd) "(%ℓ&Hcounter&#Hget&#Hupd)".
+      iIntros "Hℓ".
+      iApply "Hϕ".
+      iSplit; first done.
+      iExists _; by iFrame. }
 
-  wp.
-  iPoseProof (Stdlib__fst__spec_tac with "[//][Hϕ Hcounter]") as "H"; last iAssumption.
+    { (* Proof of the specification of [upd]. *)
+      unfold upd_spec. iIntros.
+      iIntros (ϕ) "!>(%&->&Hℓ) Hϕ".
+      wp_call.
+      iApply (Stdlib__store__spec_tac with "Hℓ[Hϕ]").
+      iNext. iIntros "Hℓ".
+      iApply "Hϕ".
+      iExists _. by iFrame. }
+  }
+  iIntros(new_counter) "#Hnew_counter". wp_continue.
 
-  wp.
-  iPoseProof (Stdlib__snd__spec_tac with "[//][Hϕ Hcounter]") as "H"; last iAssumption.
+  (* The interpreter stops at the first call of [new_couter]. This call can be
+     found in the [let () = ...] of the OCaml file. *)
+  wp_use ("Hnew_counter" with "[//][]"). iNext.
+  iIntros (vget vupd) "(%ℓ&Hℓ&#Hget&#Hupd)".
+  wp_continue.
 
-  wp.
+  wp_use Stdlib__fst__spec_tac; first done. iNext. wp_continue.
+  wp_use Stdlib__snd__spec_tac; first done. iNext. wp_continue.
 
-  iApply ("Hget" $! 0 NotStuck top with "Hcounter").
-  iNext.
-  iIntros (?)"(->&Hℓ)".
+  wp_use ("Hget" with "Hℓ").
+  iNext. iIntros (?)"[->Hℓ]".
+  wp_continue.
 
-  wp.
-  iApply ("Hupd" with "Hℓ").
+  wp_use ("Hupd" with "Hℓ").
   iNext. iIntros "Hℓ".
+  wp_continue.
 
-  wp.
-  iApply ("Hget" with "Hℓ").
-  iNext.
-  iIntros(?)"[->Hℓ]".
-  iPoseProof (Stdlib__sub__spec) as "Hsub".
-  { exact (eq_refl (VInt (int.repr 13))). }
-  { exact (eq_refl (VInt (int.repr 0))). }
-  iApply (wp_covariant with "Hsub").
-  iIntros (v)"Hv".
-  iApply (wp_covariant with "Hv"). clear v.
+  wp_use ("Hget" with "Hℓ").
+  iNext. iIntros (?)"[->Hℓ]".
+  wp_continue.
+
+  wp_use Stdlib__sub__spec;
+    [ done | done | ].
+  iIntros (vsub)"Hsub". iApply (wp_covariant with "Hsub").
   iIntros (?->).
-  iApply wp_ret.
-  iApply "Hϕ".
-  iPureIntro. reflexivity.
+
+  iClear "Hget Hupd Hℓ". clear ℓ.
+
+
+  (* The interpreter stops at the second call of [new_counter], which occurs in
+     the definition of [_test]. *)
+  wp_continue.
+  wp_use ("Hnew_counter" with "[//][]"). iNext.
+  iIntros (vget' vupd') "(%ℓ&Hℓ&#Hget&#Hupd)". wp_continue.
+
+  wp_use ("Hget" with "Hℓ").
+  iNext. iIntros (?)"[->Hℓ]".
+  wp_continue.
+
+  wp_use ("Hupd" with "Hℓ").
+  iNext. iIntros "Hℓ".
+  wp_continue.
+
+  wp_use ("Hget" with "Hℓ").
+  iNext. iIntros (?)"[->Hℓ]".
+
+  wp_use Stdlib__sub__spec;
+    [ done | done | ].
+  iIntros (vsub')"Hsub". iApply (wp_covariant with "Hsub").
+  iIntros (?->). wp_continue.
+
+  wp_specify "_test" thirteen_spec; first trivial.
+  iIntros(_test)"#H_test". wp_continue.
+
+
+  (* As all the required specifications have already been proven,
+     [wp_module_spec] will finish the proof. *)
+  wp_module_spec.
 Time Qed.
+(* With iApply everywhere 8.057 *)
